\documentclass{article}
\usepackage{amsmath}

\newcommand{\bvec}[1]{\mathbf{#1}}

\begin{document}

\thispagestyle{empty}

\begin{itemize}
\item Newton's second law of motion
\begin{eqnarray}
\bvec{a} &=& \tanh(\bvec{W}^D\bvec{x}^{D-1} + \bvec{b}^D)
\nonumber \\
\bvec{x}^l &=& \tanh(\bvec{W}^l\bvec{x}^{l-1} + \bvec{b}^l) 
\text{ for } l=1,2,\dots, D-1
\nonumber \\
\bvec{x}^0 &=& ( \bvec{m}, \bvec{x} )^t
\end{eqnarray}

\item Newton's law of universal gravitation
\begin{eqnarray}
\bvec{F} &=& \tanh(\bvec{W}^D\bvec{x}^{D-1} + \bvec{b}^D)
\nonumber \\
\bvec{x}^l &=& \tanh(\bvec{W}^l\bvec{x}^{l-1} + \bvec{b}^l) 
\text{ for } l=1,2,\dots, D-1
\nonumber \\
\bvec{x}^0 &=& (m_1, m_2, \bvec{x}_1, \bvec{x}_2)^t
\end{eqnarray}

\item Einstein's field equations
\begin{eqnarray}
\bvec{T} &=& \tanh(\bvec{W}^D\bvec{x}^{D-1} + \bvec{b}^D)
\nonumber \\
\bvec{x}^l &=& \tanh(\bvec{W}^l\bvec{x}^{l-1} + \bvec{b}^l) 
\text{ for } l=1,2,\dots, D-1
\nonumber \\
\bvec{x}^0 &=& \bvec{\rho}
\end{eqnarray}

\item Maxwell's equations
\begin{eqnarray}
(\bvec{E}, \bvec{B})^t &=& \tanh(\bvec{W}^D\bvec{x}^{D-1} + \bvec{b}^D)
\nonumber \\
\bvec{x}^l &=& \tanh(\bvec{W}^l\bvec{x}^{l-1} + \bvec{b}^l) 
\text{ for } l=1,2,\dots, D-1
\nonumber \\
\bvec{x}^0 &=& (\bvec{q}, \bvec{x}, \bvec{v})^t
\end{eqnarray}

\item Schrodinger's equation
\begin{eqnarray}
E &=& \tanh(\bvec{W}^D\bvec{x}^{D-1} + \bvec{b}^D)
\nonumber \\
\bvec{x}^l &=& \tanh(\bvec{W}^l\bvec{x}^{l-1} + \bvec{b}^l) 
\text{ for } l=1,2,\dots, D-1
\nonumber \\
\bvec{x}^0 &=& \bvec{x}
\end{eqnarray}

\item Lorentz transformation in the theory of special relativity
\begin{eqnarray}
(x', y', z', t')^t &=& \tanh(\bvec{W}^D\bvec{x}^{D-1} + \bvec{b}^D)
\nonumber \\
\bvec{x}^l &=& \tanh(\bvec{W}^l\bvec{x}^{l-1} + \bvec{b}^l) 
\text{ for } l=1,2,\dots, D-1
\nonumber \\
\bvec{x}^0 &=& (x, y, z, t, v_x, v_y, v_z)^t
\end{eqnarray}

\item Boltzmann's entropy formula
\begin{eqnarray}
S &=& \tanh(\bvec{W}^D\bvec{x}^{D-1} + \bvec{b}^D)
\nonumber \\
\bvec{x}^l &=& \tanh(\bvec{W}^l\bvec{x}^{l-1} + \bvec{b}^l) 
\text{ for } l=1,2,\dots, D-1
\nonumber \\
\bvec{x}^0 &=& (N, V, T, \bvec{m})^t \ \ (\bvec{m} \text{ encodes composition of matter})
\end{eqnarray}

\end{itemize}

\end{document}
